mechanization/lakefile.lean
@@ -7,6 +7,9 @@ require "leanprover-community" / "batteries" @ git "v4.29.0"
 
 require "leanprover-community" / "mathlib" @ git "v4.29.0"
 
+require "amarmaduke" / "lean-subst" from git
+  "https://github.com/amarmaduke/lean-subst" @ "main"
+
 require "Cedar" from git
   "https://github.com/cedar-policy/cedar-spec" @ "main" / "cedar-lean"
 
